tests/lean/run/introv.lean
@@ -1,0 +1,11 @@
+example : ∀ a b : nat, a = b → b = a :=
+begin
+  introv h,
+  exact h.symm
+end
+
+example : ∀ a b : nat, a = b → ∀ c, b = c → a = c :=
+begin
+  introv h₁ h₂,
+  exact h₁.trans h₂
+end
